\section{Integration by Parts}
\label{sec:integration-by-parts}
% Section 3.5
%\subsection{Integration By Parts}
{\bf Integration by parts}\index{Integration by parts} is an integration method which enables us to find antiderivatives of some new functions such as $\ln(x)$ as well as antiderivatives of products of functions such as $x^2\ln(x)$ and $xe^x$.

If the function we're trying to integrate can be written as a product of two functions, $u$, and $dv$, then integration by parts lets us trade out a complicated integral for hopefully simpler one.

\begin{theorem}[Integration by Parts Formula]
$$\int u\,dv=uv-\int v\,du$$
For definite integrals:
$$\int_a^bu\,dv = \left.uv\right|_a^b - \int_a^b v \,du$$
\end{theorem}
\begin{example}
Integrate $\displaystyle\int xe^x\,dx$.

\begin{solution}
To use the Integration by Parts method, we break apart the product into two parts:
$$u=x\quad \text{and}\quad dv=e^x\,dx \enspace .$$
We now calculate $du$, the derivative of $u$, and $v$, the integral of $dv$:
$$du = \left(\frac{d}{dx}x\right)\,dx \quad \text{and} \quad v = \int e^x\,dx = e^x \enspace .$$
Using the Integration by Parts formula,
$$\int xe^x\,dx = uv-\int v\,du = xe^x - \int e^x\,dx \enspace . $$
Notice the remaining integral is simpler that the original, and one which we can easily evaluate:
$$xe^x-\int e^x\,dx = xe^x - e^x + C \enspace .$$
\end{solution}\end{example}

In the last example we could have chosen either $x$ or $e^x$ as our $u$, but had we chosen $u=e^x$, the second integral would have become messier, rather than simpler.

\begin{note}[Rule of Thumb: LIATE]
When selecting the $u$ for Integration by Parts, a common rule of thumb is the ``LIATE" mnemonic. Choose $u$ in the following order of preference.
\begin{itemize}
  \item[L:] {\bf L}ogarithmic functions
  \item[I:] {\bf I}nverse trigonometric Functions
  \item[A:] {\bf A}lgebraic functions (polynomials, roots, etc.)
  \item[T:] {\bf T}rigonometic Functions
  \item[E:] {\bf E}xponential functions
\end{itemize}

\end{note}
\begin{example}
Integrate $\displaystyle\int_1^4 6x^2\ln(x)\,dx$.

\begin{solution}
Since this contains a logarithmic expression, we'll use it for our $u$.
$$u = \ln(x) \quad {\text and} \quad dv = 6x^2\,dx$$
We now calculate $du$ and $v$.
$$du = \frac{1}{x}\,dx  \quad {\text and} \quad v = \int 6x^2\,dx = 6\frac{x^3}{3} = 2x^3$$
Using the Integration By Parts formula, we have
$$\int_1^4 6x^2\ln(x)\,dx = \left.2x^3\ln(x)\right|^4_1-\int^4_1 6x^2 \frac{1}{x}\,dx \enspace .$$
We can simplify the expression in the integral on the right.
$$\int^4_1 6x^2\ln(x)\,dx = \left.2x^3\ln(x)\right|^4_1 - \int^4_1 6x\,dx$$
The remaining integral is a basic one we can now evaluate.
$$\int^4_1 6x^2\ln(x)\,dx = \left.2x^3\ln(x)\right|^4_1 - \left.3x^2\right|^4_1$$
Finally, we can evaluate the expressions.
\begin{align*}
\int^4_1 6x^2\ln(x)\,dx &= ((2\cdot 4^3\ln(4))-(2\cdot 1^3\ln(1)))-((3\cdot 4^2)-(3\cdot 1^2)) \\
&= 128\ln(4)-45\\
&\approx   132.446
\end{align*}
\end{solution}\end{example}
